Main.v
@@ -53,27 +53,24 @@ Definition linearScan
   match buildIntervals binfo oinfo blocks1 liveSets'
   return @Details blockType1 blockType2 opType1 opType2 accType maxReg with
   | inl err =>
-    Build_Details
-        _ _ _ _ _ maxReg (Some (err, BuildingIntervalsFailed))
-        liveSets' blocks1 [::] accum None None binfo oinfo
+    Build_Details _ _ _ _ _ maxReg (Some (err, BuildingIntervalsFailed))
+      liveSets' blocks1 [::] accum None None binfo oinfo
   | inr ssig =>
     (* allocate registers *)
     match walkIntervals registers_exist ssig.2 (countOps binfo blocks1).+1
     return Details maxReg with
     | inl (err, ssig') =>
-      Build_Details
-          _ _ _ _ _ maxReg (Some (err, AllocatingRegistersFailed))
-          liveSets' blocks1 [::] accum (Some ssig.1) (Some ssig'.1) binfo oinfo
+      Build_Details _ _ _ _ _ maxReg (Some (err, AllocatingRegistersFailed))
+        liveSets' blocks1 [::] accum (Some ssig.1) (Some ssig'.1) binfo oinfo
     | inr ssig' =>
-        let mappings := resolveDataFlow binfo ssig'.2 blocks1 liveSets' in
+        let allocs   := determineAllocations ssig'.1 in
+        let mappings := resolveDataFlow binfo allocs blocks1 liveSets' in
 
         (* replace virtual registers with physical registers *)
         let: (blocks2, accum') :=
-           assignRegNum binfo oinfo ssig'.2 liveSets' mappings blocks1 accum in
-        Build_Details
-            _ _ _ _ _ maxReg None
-            liveSets' blocks1 blocks2 accum' (Some ssig.1) (Some ssig'.1)
-            binfo oinfo
+           assignRegNum binfo oinfo allocs liveSets' mappings blocks1 accum in
+        Build_Details _ _ _ _ _ maxReg None liveSets' blocks1 blocks2 accum'
+          (Some ssig.1) (Some ssig'.1) binfo oinfo
     end
   end.
 
