Resolve.v
@@ -6,7 +6,6 @@ Require Import LinearScan.Interval.
 Require Import LinearScan.Blocks.
 Require Import LinearScan.LiveSets.
 Require Import LinearScan.Allocate.
-Require Import LinearScan.ScanState.
 
 Set Implicit Arguments.
 Unset Strict Implicit.
@@ -23,66 +22,67 @@ Variables blockType1 blockType2 opType1 opType2 accType : Set.
 Variable binfo : BlockInfo blockType1 blockType2 opType1 opType2.
 Variable oinfo : OpInfo maxReg accType opType1 opType2.
 
-Definition isWithin (int : IntervalDesc) (vid : nat) (knd : VarKind)
-  (opid : nat) : bool :=
-  [&& ivar int == vid
-  ,   ibeg int <= opid
-  &   if knd is Input
-      then opid <= iend int
-      else opid < iend int
-  ].
-
-Definition lookupInterval `(st : @ScanState maxReg InUse sd)
-  (vid : nat) (knd : VarKind) (opid : nat) :
-  option (IntervalId sd) :=
-  let f idx acc int := match acc with
-      | Some x => Some x
-      | None =>
-        if isWithin int.1 vid knd opid
-        then Some idx
-        else None
-      end in
-  vfoldl_with_index f None (intervals sd).
-
-Definition checkIntervalBoundary `(st : @ScanState maxReg InUse sd)
-  bid in_from from to mappings vid :=
-
-  let mfrom_int := lookupInterval st vid Output (blockLastOpId from) in
-  let mto_int   := lookupInterval st vid Input (blockFirstOpId to) in
+Definition checkIntervalBoundary (allocs : seq (Allocation maxReg))
+  (from to vid : nat) (checkIntervalKinds : bool) :
+  option (sum_eqType (ordinal_eqType maxReg) nat_eqType *
+          sum_eqType (ordinal_eqType maxReg) nat_eqType) :=
+  let mfrom_int := lookupInterval vid Output from allocs in
+  let mto_int   := lookupInterval vid Input to allocs in
 
   (* If the intervals match, no move resolution is necessary. *)
-  if mfrom_int == mto_int then mappings else
+  if option_map (@intId maxReg) mfrom_int ==
+     option_map (@intId maxReg) mto_int then None else
 
-  let f mi :=
-      if mi is Some i
-      then if lookupRegister st i is Some r
-           then inl r
-           else inr vid
-      else inr vid in
+  let f mr := if mr is Some r then inl r else inr vid in
+  let sreg := f (option_map (@intReg maxReg) mfrom_int) in
+  let dreg := f (option_map (@intReg maxReg) mto_int) in
+  if sreg == dreg
+  then None
+  else
+    if checkIntervalKinds
+    then
+      let fromk := if mfrom_int is Some i
+                   then iknd (intVal i)
+                   else Middle in
+      let tok   := if mto_int is Some i
+                   then iknd (intVal i)
+                   else Middle in
+      if match fromk, tok with
+         | LeftMost, RightMost => true
+         | LeftMost, Middle    => true
+         | Middle,   Middle    => true
+         | Middle,   RightMost => true
+         | _,        _         => false
+         end
+      then Some (sreg, dreg)
+      else None
+    else Some (sreg, dreg).
 
-  let sreg := f mfrom_int in
-  let dreg := f mto_int in
-
-  if sreg == dreg then mappings else
-
-  let addToGraphs e xs :=
-      let: (gbeg, gend) := xs in
-      if in_from
-      then (addEdge e gbeg, gend)
-      else (gbeg, addEdge e gend) in
-  let f mxs :=
-      let e := (Some sreg, Some dreg) in
-      @Some _ $ addToGraphs e
-              $ if mxs is Some xs
-                then xs
-                else (emptyGraph, emptyGraph) in
-  IntMap_alter f bid mappings.
+Definition checkBlockBoundary (allocs : seq (Allocation maxReg))
+  bid in_from from to mappings vid :=
+  if checkIntervalBoundary allocs (blockLastOpId from)
+                           (blockFirstOpId to) vid false
+    isn't Some (sreg, dreg)
+  then mappings
+  else
+    let addToGraphs e xs :=
+        let: (gbeg, gend) := xs in
+        if in_from
+        then (addEdge e gbeg, gend)
+        else (gbeg, addEdge e gend) in
+    let f mxs :=
+        let e := (Some sreg, Some dreg) in
+        @Some _ $ addToGraphs e
+                $ if mxs is Some xs
+                  then xs
+                  else (emptyGraph, emptyGraph) in
+    IntMap_alter f bid mappings.
 
 Definition BlockMoves :=
   (Graph (sum_eqType (ordinal_eqType maxReg) nat_eqType) *
    Graph (sum_eqType (ordinal_eqType maxReg) nat_eqType))%type.
 
-Definition resolveDataFlow `(st : ScanState InUse sd)
+Definition resolveDataFlow (allocs : seq (Allocation maxReg))
   (blocks : seq blockType1) (liveSets : IntMap BlockLiveSets) :
   IntMap BlockMoves :=
   (* for each block from in blocks do
@@ -123,7 +123,7 @@ Definition resolveDataFlow `(st : ScanState InUse sd)
         if IntMap_lookup s_bid liveSets isn't Some to then ms else
         let key := if in_from then bid else s_bid in
         IntSet_forFold ms (blockLiveIn to) $
-          checkIntervalBoundary st key in_from from to)
+          checkBlockBoundary allocs key in_from from to)
     (blockSuccessors binfo b).
 
 End Resolve.
